pda/pumpingLemmaTreeScript.sml
@@ -698,23 +698,6 @@ FULL_SIMP_TAC (srw_ss()) [isSubEqImpSub, isSubtree] THEN
 METIS_TAC []);
 
 
-val mapFringeLeaves = store_thm
-("mapFringeLeaves",
-``∀ptl. (∀t.t ∈ ptl ⇒ (fringe t = leaves t)) ⇒ 
- (FLAT (MAP (λa. fringe a) ptl) = cleaves ptl)``,
-
-Induct_on `ptl` THEN SRW_TAC [][leaves_def]);
-
-
-
-val fringeEqLeaves = store_thm
-("fringeEqLeaves",
-``∀t. (fringe t = leaves t)``,
-
-HO_MATCH_MP_TAC fringe_ind THEN SRW_TAC [][] THEN
-SRW_TAC [][fringe_def, leaves_def] THEN
-METIS_TAC [mapFringeLeaves]);
-
 
 val leafSubt = store_thm
 ("leafSubt",
